$$S \rarr W$$

$$W \rarr P$$

$$P \rarr C$$

$$D \rarr S$$

$$W$$

$$\rightarrowtail S$$

---

$$S \rarr W, W \rarr P, P \rarr C, D \rarr S, W \rightarrowtail S$$

$$S \rarr W, W \rarr P, P \rarr C, D \rarr S, W, \overline S \rightarrowtail$$

$$res_W \{ W, W \rarr P \} = P$$

$$res_P \{ P, P \rarr C \} = C$$

<!-- $$res_S \{ S, \overline S\} = 0$$ -->

$$res_S \{ \overline S, \overline D \lor S \} = \overline D$$

$$$$

---

$$(X \lor Y) \rarr Z \rightarrowtail X \rarr (Y \rarr Z)$$

$$(X \lor Y) \rarr Z, \overline {X \rarr (Y \rarr Z)}$$

$$(X \lor Y) \rarr Z, X \land (Y \land \overline Z)$$

$$(X \lor Y) \rarr Z, X Y \overline Z$$

$$( \overline X \land \overline Y) \lor Z, X Y \overline Z$$
